template-coq/theories/Typing.v
@@ -210,9 +210,9 @@ Inductive red1 (Σ : global_declarations) (Γ : context) : term -> term -> Prop 
 | app_red_l M1 N1 M2 : red1 Σ Γ M1 N1 -> red1 Σ Γ (tApp M1 M2) (mkApps N1 M2)
 | app_red_r M2 N2 M1 : OnOne2 (red1 Σ Γ) M2 N2 -> red1 Σ Γ (tApp M1 M2) (tApp M1 N2)
 
-| prod_red_l na na' M1 M2 N1 : red1 Σ Γ M1 N1 -> red1 Σ Γ (tProd na M1 M2) (tProd na' N1 M2)
-| prod_red_r na na' M2 N2 M1 : red1 Σ (Γ ,, vass na M1) M2 N2 ->
-                               red1 Σ Γ (tProd na M1 M2) (tProd na' M1 N2)
+| prod_red_l na M1 M2 N1 : red1 Σ Γ M1 N1 -> red1 Σ Γ (tProd na M1 M2) (tProd na N1 M2)
+| prod_red_r na M2 N2 M1 : red1 Σ (Γ ,, vass na M1) M2 N2 ->
+                               red1 Σ Γ (tProd na M1 M2) (tProd na M1 N2)
 
 | evar_red ev l l' : OnOne2 (red1 Σ Γ) l l' -> red1 Σ Γ (tEvar ev l) (tEvar ev l')
 
@@ -282,10 +282,10 @@ Lemma red1_ind_all :
        (forall (Γ : context) (p : projection) (c c' : term), red1 Σ Γ c c' -> P Γ c c' -> P Γ (tProj p c) (tProj p c')) ->
        (forall (Γ : context) (M1 N1 : term) (M2 : list term), red1 Σ Γ M1 N1 -> P Γ M1 N1 -> P Γ (tApp M1 M2) (mkApps N1 M2)) ->
        (forall (Γ : context) (M2 N2 : list term) (M1 : term), OnOne2 (fun x y => red1 Σ Γ x y /\ P Γ x y) M2 N2 -> P Γ (tApp M1 M2) (tApp M1 N2)) ->
-       (forall (Γ : context) (na na' : name) (M1 M2 N1 : term),
-        red1 Σ Γ M1 N1 -> P Γ M1 N1 -> P Γ (tProd na M1 M2) (tProd na' N1 M2)) ->
-       (forall (Γ : context) (na na' : name) (M2 N2 M1 : term),
-        red1 Σ (Γ,, vass na M1) M2 N2 -> P (Γ,, vass na M1) M2 N2 -> P Γ (tProd na M1 M2) (tProd na' M1 N2)) ->
+       (forall (Γ : context) (na : name) (M1 M2 N1 : term),
+        red1 Σ Γ M1 N1 -> P Γ M1 N1 -> P Γ (tProd na M1 M2) (tProd na N1 M2)) ->
+       (forall (Γ : context) (na : name) (M2 N2 M1 : term),
+        red1 Σ (Γ,, vass na M1) M2 N2 -> P (Γ,, vass na M1) M2 N2 -> P Γ (tProd na M1 M2) (tProd na M1 N2)) ->
        (forall (Γ : context) (ev : nat) (l l' : list term), OnOne2 (fun x y => red1 Σ Γ x y /\ P Γ x y) l l' -> P Γ (tEvar ev l) (tEvar ev l')) ->
        (forall (Γ : context) (M1 : term) (k : cast_kind) (M2 N1 : term),
         red1 Σ Γ M1 N1 -> P Γ M1 N1 -> P Γ (tCast M1 k M2) (tCast N1 k M2)) ->
